fairness/locales_helpers.v
@@ -50,6 +50,15 @@ Section XX.
     - apply locales_of_list_from_locale_from. 
   Qed.
 
+  Lemma locales_of_cfg_step `{EqDecision (expr Λ)} c1 τ c2
+    (STEP: locale_step c1 (Some τ) c2):
+    τ ∈ locales_of_cfg c1.
+  Proof using.
+    apply locale_step_from_locale_src in STEP.
+    eapply locales_of_cfg_Some; eauto.
+    Unshelve. apply c1. 
+  Qed.
+
   Definition step_fork (c1 c2: cfg Λ): option (locale Λ) :=
     let diff := locales_of_cfg c2 ∖ locales_of_cfg c1 in
     gset_pick diff. 
