lawyer/nonblocking/wfree_traces.v
@@ -1,0 +1,107 @@
+From iris.proofmode Require Import tactics.
+From fairness Require Import locales_helpers.
+From lawyer.nonblocking Require Import trace_context.
+From heap_lang Require Import lang notation.
+
+
+Close Scope Z. 
+
+
+Section UnderCtx.
+
+  (* TODO: move *)
+  Definition under_ctx (K: ectx heap_lang) (e: expr): option expr.
+  Admitted.
+
+  Lemma under_ctx_spec K e e':
+    under_ctx K e = Some e' <-> ectx_fill K e' = e.
+  Proof using. Admitted.
+
+  Lemma under_ctx_fill K e:
+    under_ctx K (ectx_fill K e) = Some e.
+  Proof using. Admitted. 
+
+End UnderCtx.
+
+
+Section CallInTrace.
+
+  Context (ic: @trace_ctx heap_lang).
+  Let ii := tctx_index ic.
+  Let Ki := tctx_ctx ic.
+  Let τi := tctx_tid ic.
+
+  Definition runs_call (ec: expr) (c: cfg heap_lang): Prop :=
+    exists e, from_locale c.1 τi = Some e /\ under_ctx Ki e = Some ec /\ to_val ec = None.
+
+  Context (m: val) (ai: val). 
+
+  Definition fits_inf_call (etr: execution_trace heap_lang): Prop :=
+    from_option (runs_call (m ai)) True (etr !! ii) /\
+    forall j, ii <= j -> from_option (fun c => exists ec, runs_call ec c) True (etr !! j).
+
+  Lemma fits_inf_call_last_or_short etr
+    (FITS: fits_inf_call etr):
+    (exists ec, runs_call ec (trace_last etr)) \/ trace_length etr <= ii. 
+  Proof using.
+    edestruct Nat.lt_ge_cases as [LT| ]; [| by eauto].
+    red in FITS. apply proj2 in FITS. red in LT.
+    ospecialize * (FITS (trace_length etr - 1)).
+    { lia. }
+    rewrite trace_lookup_last in FITS.
+    2: { lia. }
+    simpl in FITS. by left.
+  Qed.
+
+  Lemma fits_inf_call_prev etr τ c
+    (FITS: fits_inf_call (etr :tr[τ]: c)):
+    fits_inf_call etr.
+  Proof using.
+    assert (forall j cj, etr !! j = Some cj -> (etr :tr[ τ ]: c) !! j = Some cj) as LOOKUP.
+    { intros. simpl.
+      rewrite trace_lookup_extend_lt; [done| ]. 
+      by apply trace_lookup_lt_Some. }
+    red.
+    destruct FITS as [II FITS]. split.
+    { destruct (etr !! ii) eqn:ITH; rewrite ITH; [| done].
+      apply LOOKUP in ITH.
+      by rewrite ITH in II. }
+    intros ? LE.
+    specialize (FITS _ LE).
+    destruct (etr !! j) eqn:JTH; rewrite JTH; [| by eauto]. simpl.
+    apply LOOKUP in JTH.
+    by rewrite JTH in FITS. 
+  Qed.
+
+  Lemma runs_call_helper t1 t2 e ec σ
+    (EQ: τi = locale_of t1 e)
+    (RUNS: runs_call ec (t1 ++ e :: t2, σ)):
+    under_ctx Ki e = Some ec /\ to_val ec = None.
+  Proof using.
+    red in RUNS. destruct RUNS as (e_ & TIth & CUR & NVAL).
+    simpl in TIth.
+    pose proof (from_locale_from_Some [] (t1 ++ e :: t2) t1 e) as X.
+    ospecialize (X _).
+    { apply prefixes_from_spec. eauto. }
+    simpl in X. rewrite EQ /from_locale in TIth. 
+    rewrite TIth in X. inversion X. subst. eauto.
+  Qed.
+
+  Lemma fic_has_τi etr
+    (FITS : fits_inf_call etr)
+    (LEN: ii < trace_length etr):
+    τi ∈ locales_of_cfg (trace_last etr).
+  Proof using.
+    red in FITS. 
+    destruct FITS as [_ NEXT].
+    ospecialize (NEXT (trace_length etr - 1) _).
+    { lia. }
+    rewrite trace_lookup_last in NEXT.
+    2: { lia. }
+    simpl in NEXT. rewrite /runs_call in NEXT.
+    destruct NEXT as (?&?&IN&?).
+    eapply locales_of_cfg_Some; eauto.
+    Unshelve. exact inhabitant.
+  Qed.
+
+End CallInTrace. 
